commit

Bidir.v
@@ -8,38 +8,47 @@ Require Import Coq.Program.Equality.
 Require Import Coq.Sorting.Permutation.
 Require List.
 
-Inductive is_bidir_syn : forall {a : nat}, context a -> sterm a -> type -> constraints -> Prop :=
-| bidir_abs {n} ty1 gamma (st : sterm (S n)) ty2 const :
-  is_bidir_syn (gamma :: ty1) st ty2 const -> 
-  is_bidir_syn  gamma (SAbs st) (TImp ty1 ty2) const
-| bidir_cir {n} (a : nat) gamma (ct : cterm n) const :
-  is_bidir_chk gamma ct (TVar a) const ->
-  is_bidir_syn gamma (SCir a ct) (TVar a) const
-
-with is_bidir_chk : forall {a : nat}, context a -> cterm a -> type -> constraints -> Prop :=
-| bidir_var ty : is_bidir_chk [ty] CVar ty List.nil
-| bidir_app {n m} gamma delta (ct1 : cterm n) (st2 : sterm m) ty1 ty2 const1 const2 :
-  is_bidir_chk gamma ct1 (TImp ty1 ty2) const1 ->
-  is_bidir_syn delta st2 ty1 const2 ->
-  is_bidir_chk (gamma ++ delta) (CApp ct1 st2) ty2 (List.app const2 const1)
-| bidir_squ {n} gamma (st : sterm n) ty1 ty2 const :
-  is_bidir_syn gamma st ty1 const ->
-  is_bidir_chk gamma (CSqu st) ty2 (List.cons (ty1, ty2) const).
-
-Inductive is_bidir : forall {a : nat}, context a -> lterm a -> type -> constraints -> Prop :=
-| Sbidir {n} gamma (st : sterm n) ty const :
-  is_bidir_syn gamma st ty const ->
-  is_bidir gamma (LSyn st) ty const
-| Cbidir {n} gamma (ct : cterm n) ty const :
-  is_bidir_chk gamma ct ty const ->
-  is_bidir gamma (LChk ct) ty const.
-
 Inductive sat_xi : s_rules -> constraints -> Prop :=
 | sat_nil sigma : sat_xi sigma List.nil
 | sat_cons sigma ty1 ty2 const :
   sat_xi sigma const ->
   subst_ty sigma ty1 = subst_ty sigma ty2 ->
   sat_xi sigma (List.cons (ty1, ty2) const).
+
+(* -- taut -- *)
+
+Inductive is_taut : constraints -> Prop :=
+| taut_nil : is_taut List.nil
+| taut_cons ty1 ty2 const :
+  is_taut const -> ty1 = ty2 ->
+  is_taut ((ty1, ty2) :: const)%list.
+
+Lemma nil_sat_taut : forall (const : constraints),
+  sat_xi List.nil const -> is_taut const.
+Proof.
+intros const h.
+dependent induction h.
+apply taut_nil.
+simpl in H.
+apply taut_cons.
+apply IHh.
+apply JMeq_refl.
+apply H.
+Qed.
+
+Lemma taut_sat_xi : forall (sigma : s_rules) (const : constraints),
+  is_taut const -> sat_xi sigma const.
+Proof.
+intros sigma const h.
+induction h.
+- apply sat_nil.
+- rewrite H.
+  apply sat_cons.
+  apply IHh.
+  reflexivity.
+Qed.
+
+(* -- *)
 
 Lemma app_sat_xi : forall (sigma : s_rules) (const1 const2 : constraints),
   sat_xi sigma const1 -> sat_xi sigma const2 -> sat_xi sigma (const1 ++ const2)%list.
@@ -85,6 +94,31 @@ Lemma extra_sat_xi : forall (sigma : s_rules) (x : type_eq) (const : constraints
   sat_xi sigma (x :: const)%list -> sat_xi sigma const.
 Proof. intros. dependent destruction H. apply H. Qed.
 
+Lemma split_sat_xi : forall (sigma : s_rules) (const1 const2 : constraints),
+  sat_xi sigma (const1 ++ const2)%list -> sat_xi sigma const1 /\ sat_xi sigma const2.
+Proof.
+intros.
+split.
+---
+induction const2.
+- rewrite List.app_nil_r in H.
+  apply H.
+- apply IHconst2.
+  assert (sat_xi sigma (a :: const1 ++ const2)%list).
+  apply perm_sat_xi with (const1 := (const1 ++ a :: const2)%list).
+  apply Permutation_sym.
+  apply Permutation_middle.
+  apply H.
+  apply extra_sat_xi with (x := a).
+  apply H0.
+---
+induction const1; simpl in H.
+- apply H.
+- apply IHconst1.
+  apply extra_sat_xi with (x := a).
+  apply H.
+Qed.
+
 Lemma appleft_sat_xi : forall (sigma : s_rules) (const1 const2 : constraints),
   sat_xi sigma (List.app const1 const2) -> sat_xi sigma const1.
 Proof.
@@ -112,6 +146,44 @@ induction const1.
   apply extra_sat_xi with (x := a).
   apply h.
 Qed.
+
+(* ===== *)
+
+Definition is_mgu (sigma : s_rules) (const : constraints) : Prop :=
+  sat_xi sigma const /\
+  forall (sigma' : s_rules),
+    sat_xi sigma' const ->
+    exists (tau : s_rules),
+      forall (ty : type),
+        subst_ty sigma' ty = subst_ty tau (subst_ty sigma ty).
+
+(* -- bidir -- *)
+
+Inductive is_bidir_syn : forall {a : nat}, context a -> sterm a -> type -> constraints -> Prop :=
+| bidir_abs {n} ty1 gamma (st : sterm (S n)) ty2 const :
+  is_bidir_syn (gamma :: ty1) st ty2 const -> 
+  is_bidir_syn  gamma (SAbs st) (TImp ty1 ty2) const
+| bidir_cir {n} (a : nat) gamma (ct : cterm n) const :
+  is_bidir_chk gamma ct (TVar a) const ->
+  is_bidir_syn gamma (SCir a ct) (TVar a) const
+
+with is_bidir_chk : forall {a : nat}, context a -> cterm a -> type -> constraints -> Prop :=
+| bidir_var ty : is_bidir_chk [ty] CVar ty List.nil
+| bidir_app {n m} gamma delta (ct1 : cterm n) (st2 : sterm m) ty1 ty2 const1 const2 :
+  is_bidir_chk gamma ct1 (TImp ty1 ty2) const1 ->
+  is_bidir_syn delta st2 ty1 const2 ->
+  is_bidir_chk (gamma ++ delta) (CApp ct1 st2) ty2 (List.app const1 const2)
+| bidir_squ {n} gamma (st : sterm n) ty1 ty2 const :
+  is_bidir_syn gamma st ty1 const ->
+  is_bidir_chk gamma (CSqu st) ty2 (List.cons (ty1, ty2) const).
+
+Inductive is_bidir : forall {a : nat}, context a -> lterm a -> type -> constraints -> Prop :=
+| Sbidir {n} gamma (st : sterm n) ty const :
+  is_bidir_syn gamma st ty const ->
+  is_bidir gamma (LSyn st) ty const
+| Cbidir {n} gamma (ct : cterm n) ty const :
+  is_bidir_chk gamma ct ty const ->
+  is_bidir gamma (LChk ct) ty const.
 
 Theorem bidir_typed_syn :
   forall {n : nat} (gamma : context n) (st : sterm n) (ty : type) (const : constraints) (sigma : s_rules),
@@ -148,14 +220,14 @@ Proof.
     with (ty1 := (subst_ty sigma ty1)).
     * rewrite <- dist_subst_ty.
       apply IHhb.
-      apply appright_sat_xi
-      with (const1 := const2).
+      apply appleft_sat_xi
+      with (const2 := const2).
       apply hs.
     * apply bidir_typed_syn
       with (const := const2).
       apply H.
-      apply appleft_sat_xi
-      with (const2 := const1).
+      apply appright_sat_xi
+      with (const1 := const1).
       apply hs.
   + simpl.
     dependent destruction hs.
@@ -164,3 +236,103 @@ Proof.
     with (const := const).
     apply H. apply hs.
 Qed.
+
+(* -- inter -- *)
+
+Inductive is_inter_syn : forall {a : nat}, context a -> sterm a -> type -> Prop :=
+| inter_abs {n} ty1 gamma (st : sterm (S n)) ty2 :
+  is_inter_syn (gamma :: ty1) st ty2 -> 
+  is_inter_syn  gamma (SAbs st) (TImp ty1 ty2)
+| inter_cir {n} (a : nat) gamma (ct : cterm n) sigma :
+  is_inter_chk gamma ct (TVar a) sigma ->
+  is_inter_syn (subst_ctx sigma gamma) (SCir a ct) (subst_ty sigma (TVar a))
+
+with is_inter_chk : forall {a : nat}, context a -> cterm a -> type -> s_rules -> Prop :=
+| inter_var ty : is_inter_chk [ty] CVar ty List.nil
+| inter_app {n m} gamma delta (ct1 : cterm n) (st2 : sterm m) ty1 ty2 sigma :
+  is_inter_chk gamma ct1 (TImp ty1 ty2) sigma ->
+  is_inter_syn delta st2 ty1 ->
+  is_inter_chk (gamma ++ delta) (CApp ct1 st2) ty2 sigma
+| inter_squ {n} gamma (st : sterm n) ty1 ty2 sigma :
+  is_inter_syn gamma st ty1 ->
+  is_mgu sigma ((ty1, ty2) :: List.nil)%list ->
+  is_inter_chk gamma (CSqu st) ty2 sigma.
+
+Inductive is_inter : forall {a : nat}, context a -> lterm a -> type -> Prop :=
+| Sinter {n} gamma (st : sterm n) ty :
+  is_inter_syn gamma st ty ->
+  is_inter gamma (LSyn st) ty
+| Cinter {n} gamma (ct : cterm n) ty :
+  is_inter_chk gamma ct ty List.nil ->
+  is_inter gamma (LChk ct) ty.
+
+Theorem inter_typed_syn :
+  forall {n : nat} (gamma : context n) (st : sterm n) (ty : type),
+  is_inter_syn gamma st ty ->
+  is_typed gamma (strip_syn st) ty
+
+with inter_typed_chk :
+  forall {n : nat} (gamma : context n) (ct : cterm n) (ty : type) (sigma : s_rules),
+  is_inter_chk gamma ct ty sigma ->
+  is_typed (subst_ctx sigma gamma) (strip_chk ct) (subst_ty sigma ty).
+
+Proof.
+- intros n gamma st ty h.
+  induction h.
+  + simpl.
+    apply typed_abs.
+    apply IHh.
+  + simpl.
+    apply inter_typed_chk.
+    apply H.
+- intros n gamma st ty sigma h.
+  induction h.
+  + simpl. apply typed_var.
+  + simpl.
+    rewrite app_subst_ctx.
+    apply typed_app with (ty1 := subst_ty sigma ty1).
+    * rewrite <- dist_subst_ty.
+      apply IHh.
+    * apply subst_typed.
+      apply inter_typed_syn.
+      apply H.
+  + simpl.
+    destruct H0.
+    dependent destruction H0.
+    rewrite <- H1.
+    apply subst_typed.
+    apply inter_typed_syn.
+    apply H.
+Qed.
+
+
+
+
+
+
+
+
+
+
+
+
+
+
+
+
+
+
+
+
+
+
+
+
+
+
+
+
+
+
+
+
