Workbench.v
@@ -7,529 +7,267 @@ Require Import Types.
 Require Import Subst.
 Require Import LabeledLambda.
 Require Import Bidir.
+Require Import Build.
 
 Require Import Coq.Program.Equality.
 Require Import Coq.Sorting.Permutation.
 Require Import Arith.
 Require List.
 
+(* -- *)
 
-Inductive not_FTV : nat -> type -> Prop :=
-| nFTV_var a b : a <> b -> not_FTV a (TVar b)
-| nFTV_imp a ty1 ty2 :
-  not_FTV a ty1 ->
-  not_FTV a ty2 ->
-  not_FTV a (TImp ty1 ty2).
+(* -- Princ -- *)
 
 (*
-Inductive not_FCV_syn : forall {n : nat}, nat -> sterm n -> Prop :=
-| nFCV_abs st : not_FCV_syn st -> not_FCV_syn (SAbs st)
-| nFCV_cir a ct : 
+Definition is_princ {n : nat} (gamma : context n) (pt : pterm n) (ty : type) : Prop :=
+  is_typed gamma pt ty /\
+  forall (gamma' : context n) (ty' : type),
+  is_typed gamma' pt ty' ->
+  (exists (sigma : s_rules), gamma' = subst_ctx sigma gamma) ->
+  (exists (sigma : s_rules), gamma' = subst_ctx sigma gamma /\ ty' = subst_ty sigma ty).
 *)
-
-(* Unique Atomic Names *)
-
-Fixpoint uniq_circ_syn {n : nat} (t : sterm n) (a : nat) : (sterm n * nat) :=
-match t with
-| SAbs t' => 
-  let (tnew, a') := uniq_circ_syn t' a in
-  (SAbs tnew, a')
-| SCir _ t' =>
-  let (tnew, a') := uniq_circ_chk t' (S a) in
-  (SCir a tnew, a')
-end
-with uniq_circ_chk {n : nat} (t : cterm n) (a : nat) : (cterm n * nat) :=
-match t with
-| CVar => (CVar, a)
-| CApp t1 t2 =>
-  let (tnew1, a1) := uniq_circ_chk t1 a in
-  let (tnew2, a2) := uniq_circ_syn t2 a1 in
-  (CApp tnew1 tnew2, a2)
-| CSqu t' =>
-  let (tnew, a') := uniq_circ_syn t' a in
-  (CSqu tnew, a')
-end.
-
-Definition uniq_circ {n : nat} (t : lterm n) : lterm n :=
-match t with
-| LSyn st => let (res, _) := uniq_circ_syn st 0 in LSyn res
-| LChk ct => let (res, _) := uniq_circ_chk ct 0 in LChk res
-end.
 
 (*
-Inductive is_uniq_syn : forall {n : nat}, sterm n -> Prop :=
-| uniq_abs st : is_uniq_syn st -> is_uniq_syn (SAbs st)
-| uniq_cir a ct :
-  is_uniq_chk ct ->
-  (* not_FTV a ct -> *)
-  is_uniq_syn (SCir a ct)
-
-with is_uniq_chk : forall {n : nat}, cterm n -> Prop :=
-| uniq_var : is_uniq_chk CVar
-| uniq_app ct1 st2 :
-  is_uniq_chk ct1 ->
-  is_uniq_syn st2 ->
+Definition is_princ {n : nat} (gamma : context n) (pt : pterm n) (ty : type) : Prop :=
+  is_typed gamma pt ty /\
+  forall (ty' : type),
+  is_typed gamma pt ty' ->
+  exists (sigma : s_rules),
+  ty' = subst_ty sigma ty.
 *)
 
-(* Tautology *)
+Definition is_princ {n : nat} (gamma : context n) (pt : pterm n) (ty : type) : Prop :=
+  is_typed gamma pt ty /\
+  forall (gamma' : context n) (ty' : type),
+  is_typed gamma' pt ty' ->
+  exists (sigma : s_rules),
+  gamma' = subst_ctx sigma gamma /\ ty' = subst_ty sigma ty.
 
-Inductive is_taut : constraints -> Prop :=
-| taut_nil : is_taut List.nil
-| taut_cons ty1 ty2 const :
-  is_taut const -> ty1 = ty2 ->
-  is_taut ((ty1, ty2) :: const)%list.
-
-Lemma nil_sat_taut : forall (const : constraints),
-  sat_xi List.nil const -> is_taut const.
-Proof.
-intros const h.
-dependent induction h.
-apply taut_nil.
-simpl in H.
-apply taut_cons.
-apply IHh.
-apply JMeq_refl.
-apply H.
-Qed.
-
-Lemma taut_sat_xi : forall (sigma : s_rules) (const : constraints),
-  is_taut const -> sat_xi sigma const.
-Proof.
-intros sigma const h.
-induction h.
-- apply sat_nil.
-- rewrite H.
-  apply sat_cons.
-  apply IHh.
-  reflexivity.
-Qed.
-
-(* Planar Lambda Typing Properties *)
-
-Inductive good_rule : s_rule -> Prop :=
-| good_id a : good_rule (a, TVar a)
-| good_nFTV a ty :
-  not_FTV a ty ->
-  good_rule (a, ty).
-
-Inductive good_rules : s_rules -> Prop :=
-| good_nil : good_rules List.nil
-| good_cons rul sigma :
-  good_rule rul ->
-  good_rules sigma ->
-  good_rules (rul :: sigma)%list.
-
-Lemma subst1_ty_nFTV : forall (a : nat) (ty ty' : type),
-  not_FTV a ty -> subst1_ty (a, ty') ty = ty.
-Proof.
-intros a ty ty' h.
-induction h.
-- simpl.
-  case_eq (b =? a).
-  + intro eq. apply Nat.eqb_eq in eq.
-    apply eq_sym in eq. apply H in eq.
-    contradiction.
-  + reflexivity.
-- simpl.
-  rewrite IHh1.
-  rewrite IHh2.
-  reflexivity.
-Qed.
-
-Lemma subst1_ty_idem : forall (rul : s_rule) (ty : type),
-  good_rule rul ->
-  subst1_ty rul (subst1_ty rul ty) = subst1_ty rul ty.
-Proof.
-intros rul ty h.
-induction h; induction ty.
-- simpl.
-  case_eq (n =? a); intro eq; simpl.
-  + case_eq (a =? a); reflexivity.
-  + rewrite eq. reflexivity.
-- simpl. rewrite IHty1. rewrite IHty2.
-  reflexivity.
-- simpl.
-  case_eq (n =? a); intro eq.
-  + apply subst1_ty_nFTV.
-    apply H.
-  + simpl. rewrite eq.
-    reflexivity.
-- simpl.
-  rewrite IHty1.
-  rewrite IHty2.
-  reflexivity.
-Qed.
-
-Lemma subst1_ty_id : forall (a : nat) (ty : type),
-  good_rule (a, ty) ->
-  ty = subst1_ty (a, ty) ty.
-Proof.
-intros a ty h.
-dependent induction h.
-- simpl. case (a =? a); reflexivity.
-- rewrite subst1_ty_nFTV. reflexivity.
-  apply H.
-Qed.
-
-Lemma subst1_const_nil : forall (rul : s_rule) (const : constraints),
-  subst1_const rul const = List.nil ->
-  const = List.nil.
-Proof.
-intros rul const h.
-induction const.
-- reflexivity.
-- assert
-  (List.length (subst1_const rul (a :: const)%list) =
-   List.length Datatypes.nil (A := type_eq)).
-  rewrite h. reflexivity.
-  destruct a.
-  simpl in H.
-  discriminate.
-Qed.
-
-Lemma subst_sat_xi : forall (sigma : s_rules) (const : constraints) (a : nat) (ty : type),
-  sat_xi sigma (subst1_const (a, ty) const) ->
-  sat_xi ((a, ty) :: sigma)%list const.
-Proof.
-intros sigma const a ty h.
-induction const.
-- apply sat_nil.
-- destruct a0. apply sat_cons.
-  + apply IHconst.
-    apply extra_sat_xi with
-    (x := (subst1_ty (a, ty) t, subst1_ty (a, ty) t0)).
-    simpl in h. apply h.
-  + simpl.
-    simpl in h.
-    dependent destruction h.
-    apply H.
-Qed.
-
-Inductive build_subst : s_rules -> constraints -> Prop :=
-| build_nil : build_subst List.nil List.nil
-| build_consleft sigma const a ty :
-  build_subst sigma (subst1_const (a, ty) const) ->
-  build_subst ((a, ty) :: sigma)%list ((TVar a, ty) :: const)%list
-| build_consright sigma const b ty :
-  build_subst sigma (subst1_const (b, ty) const) ->
-  build_subst ((b, ty) :: sigma)%list ((ty, TVar b) :: const)%list
-| build_consimp rul sigma const tyA tyB tyC tyD :
-  build_subst (rul :: sigma)%list ((tyC, tyA) :: (tyB, tyD) :: const)%list ->
-  build_subst (rul :: sigma)%list ((TImp tyA tyB, TImp tyC tyD) :: const)%list.
-
-Lemma build_sat : forall (sigma : s_rules) (const : constraints),
-  build_subst sigma const ->
-  good_rules sigma ->
-  sat_xi sigma const.
-Proof.
-intros sigma const h good.
-induction h.
-- apply sat_nil.
-- dependent destruction good.
-  apply sat_cons.
-  + apply subst_sat_xi.
-    apply IHh. apply good.
-  + dependent destruction H.
-* reflexivity.
-* simpl.
-  case_eq (a =? a); intro eq.
-  -- rewrite <- subst1_ty_id.
-     reflexivity.
-     apply good_nFTV. apply H.
-  -- rewrite Nat.eqb_refl in eq.
-     apply Bool.diff_true_false in eq.
-     contradiction.
-- dependent destruction good.
-  apply sat_cons.
-  + apply subst_sat_xi.
-    apply IHh. apply good.
-  + dependent destruction H.
-* reflexivity.
-* simpl.
-  case_eq (b =? b); intro eq.
-  -- rewrite <- subst1_ty_id.
-     reflexivity.
-     apply good_nFTV. apply H.
-  -- rewrite Nat.eqb_refl in eq.
-     apply Bool.diff_true_false in eq.
-     contradiction.
-- assert (sat_xi (rul :: sigma)%list ((tyC, tyA) :: (tyB, tyD) :: const)%list).
-  apply IHh. apply good.
-  apply sat_cons.
-  + apply extra_sat_xi with (x := (tyB, tyD)).
-    apply extra_sat_xi with (x := (tyC, tyA)).
-    apply H.
-  + dependent destruction H.
-    dependent destruction H.
-    rewrite ? dist_subst_ty.
-    rewrite H0. rewrite H1.
-    reflexivity.
-Qed.
-
-Lemma build_app : forall (const1 const2 : constraints) (sigma : s_rules) ,
-  build_subst sigma (const2 ++ const1)%list ->
-  exists sigma2 sigma1 : s_rules,
-  build_subst sigma2 const2 /\
-  build_subst sigma1 const1 /\
-  sigma = (sigma2 ++ sigma1)%list.
-Proof.
-intros const1 const2.
-induction const2; intros sigma h.
-- exists List.nil. exists sigma.
-  split. apply build_nil.
-  split. simpl in h. apply h.
-  simpl. reflexivity.
-- simpl in h.
-  dependent destruction h.
-  + assert (
-      exists sigma2 sigma1 : s_rules,
-      build_subst sigma2 (subst1_const (a0, ty) const2) /\
-      build_subst sigma1 const1 /\ sigma = (sigma2 ++ sigma1)%list
-    ). admit.
-    destruct H.
-    destruct H.
-    destruct H.
-    destruct H0.
-    exists ((a0, ty) :: x)%list.
-    exists x0.
-    split. apply build_consleft. apply H.
-    split. apply H0.
-    simpl. rewrite H1. reflexivity.
-Admitted.
+(* -- Bidir -- *)
 
 (*
-
-  assert (
-      exists sigma2 sigma1 : s_rules,
-      build_subst sigma2 const2 /\
-      build_subst sigma1 const1 /\ ((a0, ty) :: sigma)%list = (sigma2 ++ sigma1)%list
-    ). apply IHconst2.
-    destruct const2.
-    destruct const1.
-    simpl in h. simpl. dependent destruction.
-    
-
-  assert (
-    exists sigma2 sigma1 : s_rules,
-    build_subst sigma2 const2 /\
-    build_subst sigma1 const1 /\ sigma = (sigma2 ++ sigma1)%list
-  ).
-  apply IHconst2.
-
-
-  dependent destruction h.
-  + assert (
-      exists sigma2 sigma1 : s_rules,
-      build_subst sigma2 const2 /\
-      build_subst sigma1 const1 /\ ((a0, ty) :: sigma)%list = (sigma2 ++ sigma1)%list
-    ).
-    apply IHconst2.
-    apply build_consleft.
-
-  
-
-destruct const2; destruct const1.
-- exists List.nil. exists List.nil.
-  split. apply build_nil. split. apply build_nil.
-  simpl. simpl in h.
-  dependent destruction h.
-  reflexivity.
-- simpl in h.
-  exists List.nil. exists sigma.
-  split. apply build_nil.
-  split. apply h.
-  simpl. reflexivity.
-- simpl in h. rewrite List.app_nil_r in h.
-  exists sigma. exists List.nil.
-  split. apply h.
-  split. apply build_nil.
-  rewrite List.app_nil_r.
-  reflexivity.
-- assert (
-    exists sigma2 sigma1 : s_rules,
-    build_subst sigma2 const2 /\
-    build_subst sigma1 (t0 :: const1)%list /\ sigma = (sigma2 ++ sigma1)%list
-  ).
-  
-
-
-dependent induction h.
-- dependent destruction const2.
-  dependent destruction const1.
-  exists List.nil.
-  exists List.nil.
-  split. apply build_nil.
-  split. apply build_nil.
-  simpl. reflexivity.
-  simpl in x. discriminate.
-  simpl in x. discriminate.
-- 
-Admitted.
-*)
-
-Lemma good_app : forall (sigma1 sigma2 : s_rules),
-  good_rules sigma1 -> good_rules sigma2 -> good_rules (sigma1 ++ sigma2)%list.
-Proof.
-intros sigma1 sigma2 h1 h2.
-induction h1.
-- simpl. apply h2.
-- simpl. apply good_cons.
-  apply H. apply IHh1.
-Qed.
-
-Lemma build_bidir_good_syn :
-  forall {n : nat} (gamma : context n) (st : sterm n)
-  (ty : type) (const : constraints) (sigma : s_rules),
+Theorem bidir_princ_syn :
+  forall {n : nat} (gamma : context n) (st : sterm n) (ty : type) (const : constraints) (sigma : s_rules),
   is_bidir_syn gamma st ty const ->
-  build_subst sigma const ->
-  good_rules sigma
-
-with build_bidir_good_chk :
-  forall {n : nat} (gamma : context n) (ct : cterm n)
-  (ty : type) (const : constraints) (sigma : s_rules),
-  is_bidir_chk gamma ct ty const ->
-  build_subst sigma const ->
-  good_rules sigma.
-
+  is_mgu sigma const ->
+  is_princ (subst_ctx sigma gamma) (strip_syn st) (subst_ty sigma ty).
 Proof.
-- intros n gamma st ty const sigma hb h.
-  dependent induction hb.
-  + apply IHhb. apply h.
-  + apply build_bidir_good_chk with
-    (n := n) (gamma := gamma) (ct := ct)
-    (ty := (TVar a)) (const := const).
-    apply H. apply h.
-- intros n gamma st ty const sigma hb h.
-  dependent induction hb.
-  + dependent destruction h. apply good_nil.
-  + apply build_app in h.
-    destruct h.
-    destruct H0.
-    destruct H0.
-    destruct H1.
-    rewrite H2.
-    apply good_app.
-    apply build_bidir_good_syn with
-    (n := m) (gamma := delta) (st := st2)
-    (ty := ty1) (const := const2).
-    apply H. apply H0.
-    apply build_bidir_good_chk with
-    (n := n) (gamma := gamma) (ct := ct1)
-    (ty := TImp ty1 ty2) (const := const1).
-    apply hb. apply H1.
-  + admit.
+intros.
+destruct H0. split.
+--
+apply bidir_typed_syn with (const := const).
+apply H. apply H0.
+--
+intros. destruct H3.
+assert (
+  exists (sigma' : s_rules),
+  sat_xi sigma' const /\
+  ty' = subst_ty sigma' ty
+). admit. (* apply bidir_sigma_syn with (st := st). apply H. apply H2. *)
+destruct H4.
+assert (
+ exists tau : s_rules,
+ forall ty : type, subst_ty x0 ty = subst_ty tau (subst_ty sigma ty)
+). apply H1. apply H4.
+destruct H5.
+exists x0. split.
+- rewrite <- subst_forall_ctx with (sigma' := x0).
+rewrite <- H4. apply H3.
+Admitted.
+Qed.
+
+ destruct H3. split.
+rewrite H4. rewrite H5.
+assert (
+ exists tau : s_rules,
+ forall ty : type, subst_ty x ty = subst_ty tau (subst_ty sigma ty)
+). apply H1. apply H3.
+destruct H6. 
+exists x0. split.
+- apply subst_forall_ctx. apply H6.
+- apply H6.
+Qed.
+*)
+
+(*
+Lemma bidir_sigma_syn :
+  forall {n : nat} (gamma : context n) (st : sterm n) (ty : type) (const : constraints) (sigma : s_rules),
+  is_bidir_syn gamma st ty const ->
+  is_mgu sigma const ->
+  forall (ty' : type),
+  is_typed (subst_ctx sigma gamma) (strip_syn st) ty' ->
+  exists (sigma' : s_rules),
+  sat_xi sigma' const /\ ty' = subst_ty sigma' ty.
+Proof.
+intros n gamma st ty const sigma hb.
+dependent induction hb; intros hm ty' ht.
+-
+dependent destruction ht.
+
+assert (ty0 = subst_ty sigma ty1). admit.
+
+assert (
+  exists sigma' : s_rules, sat_xi sigma' const /\ ty3 = subst_ty sigma' ty2
+). apply IHhb. apply hm.
+
+rewrite cons_subst_ctx. rewrite <- H. apply ht.
+
+destruct H0. exists x.
+split. apply H0.
+rewrite dist_subst_ty.
+destruct H0.
+rewrite <- H1.
+admit.
+
+-
 Admitted.
 
-(* Principality *)
+(* ---------------- *)
 
-Inductive subst_dom : s_rules -> s_rules -> constraints -> Prop :=
-| dom_nil sigma : subst_dom sigma List.nil List.nil
-| dom_cons sigma1 sigma2 ty1 ty2 const :
-  subst_dom sigma1 sigma2 const ->
-  subst_ty sigma1 (subst_ty sigma2 ty1) = subst_ty sigma1 ty1 ->
-  subst_ty sigma1 (subst_ty sigma2 ty2) = subst_ty sigma1 ty2 ->
-  subst_dom sigma1 sigma2 ((ty1, ty2) :: const)%list.
-
-Definition is_principal (sigma : s_rules) (const : constraints) : Prop :=
-  sat_xi sigma const /\
-  (forall (sigma' : s_rules),
-   sat_xi sigma' const ->
-   forall (const' : constraints),
-   subst_dom sigma' sigma const').
-
-Lemma build_princ : forall (sigma : s_rules) (const : constraints),
-  build_subst sigma const ->
-  good_rules sigma ->
-  is_principal sigma const.
+Theorem bidir_princ_syn :
+  forall {n : nat} (gamma : context n) (st : sterm n) (ty : type) (const : constraints) (sigma : s_rules),
+  is_bidir_syn gamma st ty const ->
+  is_mgu sigma const ->
+  is_princ (subst_ctx sigma gamma) (strip_syn st) (subst_ty sigma ty).
 Proof.
-intros sigma const hb good.
+intros.
 split.
-- apply build_sat. apply hb. apply good.
-- intros sigma' hs. dependent induction hb.
-  + intros. apply dom_nil.
-  + admit.
-  + admit.
-  + admit.
+--
+destruct H0.
+apply bidir_typed_syn with (const := const).
+apply H. apply H0.
+--
+intros.
+assert (
+  exists (sigma' : s_rules),
+  sat_xi sigma' const /\
+  ty' = subst_ty sigma' ty
+). apply bidir_sigma_syn with (sigma := sigma) (gamma := gamma) (st := st).
+apply H. apply H0. apply H1.
+destruct H0.
+destruct H2. destruct H2.
+rewrite H4.
+assert (
+ exists tau : s_rules,
+ forall ty : type, subst_ty x ty = subst_ty tau (subst_ty sigma ty)
+). apply H3. apply H2.
+destruct H5. 
+exists x0.
+apply H5.
+Qed.
+*)
+
+Lemma bidir_sigma_syn :
+  forall {n : nat} (gamma : context n) (st : sterm n) (ty : type) (const : constraints),
+  is_bidir_syn gamma st ty const ->
+  forall (gamma' : context n) (ty' : type),
+  is_typed gamma' (strip_syn st) ty' ->
+  exists (sigma : s_rules),
+  sat_xi sigma const /\
+  gamma' = subst_ctx sigma gamma /\ ty' = subst_ty sigma ty.
+Proof.
+intros.
 Admitted.
 
-(* Unification *)
+(*
+dependent induction H.
 
-Inductive is_inter_syn : forall {a : nat}, context a -> sterm a -> type -> Prop :=
-| inter_abs {n} ty1 gamma (st : sterm (S n)) ty2 :
-  is_inter_syn (gamma :: ty1) st ty2 -> 
-  is_inter_syn  gamma (SAbs st) (TImp ty1 ty2)
-| inter_cir {n} (a : nat) gamma (ct : cterm n) sigma :
-  is_inter_chk gamma ct (TVar a) sigma ->
-  is_inter_syn (subst_ctx sigma gamma) (SCir a ct) (subst_ty sigma (TVar a))
 
-with is_inter_chk : forall {a : nat}, context a -> cterm a -> type -> s_rules -> Prop :=
-| inter_var ty : is_inter_chk [ty] CVar ty List.nil
-| inter_app {n m} gamma delta (ct1 : cterm n) (st2 : sterm m) ty1 ty2 sigma :
-  is_inter_chk gamma ct1 (TImp ty1 ty2) sigma ->
-  is_inter_syn delta st2 ty1 ->
-  is_inter_chk (gamma ++ delta) (CApp ct1 st2) ty2 sigma
-| inter_squ {n} gamma (st : sterm n) ty1 ty2 sigma :
-  is_inter_syn gamma st ty1 ->
-  sat_xi sigma ((ty1, ty2) :: List.nil)%list ->
-  is_inter_chk gamma (CSqu st) ty2 sigma.
+--
+assert (
+  exists sigma : s_rules,
+  sat_xi sigma const /\
+  gamma' :: ty1 = subst_ctx sigma (gamma :: ty1) /\
+  ty2 = subst_ty sigma ty2
+). apply IHis_bidir_syn. admit.
+destruct H1.
+exists x.
+split. apply H1.
+split. admit.
+rewrite dist_subst_ty. admit.
 
-Inductive is_inter : forall {a : nat}, context a -> lterm a -> type -> Prop :=
-| Sbidir {n} gamma (st : sterm n) ty :
-  is_inter_syn gamma st ty ->
-  is_inter gamma (LSyn st) ty
-| Cbidir {n} gamma (ct : cterm n) ty :
-  is_inter_chk gamma ct ty List.nil ->
-  is_inter gamma (LChk ct) ty.
+dependent destruction H0.
+*)
 
+Theorem bidir_princ_syn :
+  forall {n : nat} (gamma : context n) (st : sterm n) (ty : type) (const : constraints) (sigma : s_rules),
+  is_bidir_syn gamma st ty const ->
+  is_mgu sigma const ->
+  is_princ (subst_ctx sigma gamma) (strip_syn st) (subst_ty sigma ty).
+Proof.
+intros.
+destruct H0. split.
+apply bidir_typed_syn with (const := const).
+apply H. apply H0.
+intros.
+assert (
+  exists (sigma' : s_rules),
+  sat_xi sigma' const /\
+  gamma' = subst_ctx sigma' gamma /\ ty' = subst_ty sigma' ty
+). apply bidir_sigma_syn with (st := st). apply H. apply H2.
+destruct H3. destruct H3. destruct H4.
+rewrite H4. rewrite H5.
+assert (
+ exists tau : s_rules,
+ forall ty : type, subst_ty x ty = subst_ty tau (subst_ty sigma ty)
+). apply H1. apply H3.
+destruct H6. 
+exists x0. split.
+- apply subst_forall_ctx. apply H6.
+- apply H6.
+Qed.
+
+(* -- Inter -- *)
+
+(*
 Theorem inter_typed_syn :
   forall {n : nat} (gamma : context n) (st : sterm n) (ty : type),
   is_inter_syn gamma st ty ->
-  is_typed gamma (strip_syn st) ty
+  is_princ gamma (strip_syn st) ty
 
 with inter_typed_chk :
   forall {n : nat} (gamma : context n) (ct : cterm n) (ty : type) (sigma : s_rules),
   is_inter_chk gamma ct ty sigma ->
-  is_typed (subst_ctx sigma gamma) (strip_chk ct) (subst_ty sigma ty).
+  is_princ (subst_ctx sigma gamma) (strip_chk ct) (subst_ty sigma ty).
 
 Proof.
-- intros n gamma st ty h.
-  induction h.
-  + simpl.
-    apply typed_abs.
-    apply IHh.
-  + simpl.
-    apply inter_typed_chk.
-    apply H.
-- intros n gamma st ty sigma h.
-  induction h.
-  + simpl. apply typed_var.
-  + simpl.
-    rewrite app_subst_ctx.
-    apply typed_app with (ty1 := subst_ty sigma ty1).
-    * rewrite <- dist_subst_ty.
-      apply IHh.
-    * apply subst_typed.
-      apply inter_typed_syn.
-      apply H.
-  + simpl.
-    dependent destruction H0.
-    rewrite <- H1.
-    apply subst_typed.
-    apply inter_typed_syn.
-    apply H.
-Qed.
 
-(* Principal Typing *)
+--
+intros. split.
+apply inter_typed_syn. apply H.
 
-(*
-Inductive is_comp_sigma : s_rules -> s_rules -> Prop :=
-| comp_nil sigma : is_comp_sigma sigma List.nil
-| comp_id sigma : is_comp_sigma sigma sigma
-| comp_cons sigma :
+dependent induction H; intros.
+- 
+Admitted.
+
+
+
 *)
 
-Definition is_princ := forall {n : nat} (ctx : context n) (pt : pterm n) (ty : type),
-  is_typed ctx pt ty -> forall (ctx' : context n) (ty' : type), is_typed ctx' pt ty' ->
-  sig (fun (sigma : s_rules) => ctx' = subst_ctx sigma ctx /\ ty' = subst_ty sigma ty).
+
+
+
+
+
+
+
+
+
+
+
+
+
+
+
+
+
+
+
+
+
+
+
+
+
 
 
