Build.v
@@ -1,0 +1,461 @@
+Require Import Nat.
+Require Import Snoclist.
+Import SnoclistNotations.
+Require Import PlanarLambda.
+Require Import Types.
+
+Require Import Subst.
+Require Import LabeledLambda.
+Require Import Bidir.
+
+Require Import Coq.Program.Equality.
+Require Import Coq.Sorting.Permutation.
+Require Import Arith.
+Require List.
+
+Inductive good_rule : s_rule -> Prop :=
+| good_id a : good_rule (a, TVar a)
+| good_nFTV a ty :
+  not_FTV a ty ->
+  good_rule (a, ty).
+
+Inductive good_rules : s_rules -> Prop :=
+| good_nil : good_rules List.nil
+| good_cons rul sigma :
+  good_rule rul ->
+  good_rules sigma ->
+  good_rules (rul :: sigma)%list.
+
+Lemma good_app : forall (sigma1 sigma2 : s_rules),
+  good_rules sigma1 -> good_rules sigma2 -> good_rules (sigma1 ++ sigma2)%list.
+Proof.
+intros sigma1 sigma2 h1 h2.
+induction h1.
+- simpl. apply h2.
+- simpl. apply good_cons.
+  apply H. apply IHh1.
+Qed.
+
+Lemma subst1_ty_nFTV : forall (a : nat) (ty ty' : type),
+  not_FTV a ty -> subst1_ty (a, ty') ty = ty.
+Proof.
+intros a ty ty' h.
+induction h.
+- simpl.
+  case_eq (b =? a).
+  + intro eq. apply Nat.eqb_eq in eq.
+    apply eq_sym in eq. apply H in eq.
+    contradiction.
+  + reflexivity.
+- simpl.
+  rewrite IHh1.
+  rewrite IHh2.
+  reflexivity.
+Qed.
+
+Lemma subst1_ty_idem : forall (rul : s_rule) (ty : type),
+  good_rule rul ->
+  subst1_ty rul (subst1_ty rul ty) = subst1_ty rul ty.
+Proof.
+intros rul ty h.
+induction h; induction ty.
+- simpl.
+  case_eq (n =? a); intro eq; simpl.
+  + case_eq (a =? a); reflexivity.
+  + rewrite eq. reflexivity.
+- simpl. rewrite IHty1. rewrite IHty2.
+  reflexivity.
+- simpl.
+  case_eq (n =? a); intro eq.
+  + apply subst1_ty_nFTV.
+    apply H.
+  + simpl. rewrite eq.
+    reflexivity.
+- simpl.
+  rewrite IHty1.
+  rewrite IHty2.
+  reflexivity.
+Qed.
+
+Lemma subst1_ty_id : forall (a : nat) (ty : type),
+  good_rule (a, ty) ->
+  ty = subst1_ty (a, ty) ty.
+Proof.
+intros a ty h.
+dependent induction h.
+- simpl. case (a =? a); reflexivity.
+- rewrite subst1_ty_nFTV. reflexivity.
+  apply H.
+Qed.
+
+Lemma subst1_const_nil : forall (rul : s_rule) (const : constraints),
+  subst1_const rul const = List.nil ->
+  const = List.nil.
+Proof.
+intros rul const h.
+induction const.
+- reflexivity.
+- assert
+  (List.length (subst1_const rul (a :: const)%list) =
+   List.length Datatypes.nil (A := type_eq)).
+  rewrite h. reflexivity.
+  destruct a.
+  simpl in H.
+  discriminate.
+Qed.
+
+Lemma subst_sat_xi : forall (sigma : s_rules) (const : constraints) (a : nat) (ty : type),
+  sat_xi sigma (subst1_const (a, ty) const) ->
+  sat_xi ((a, ty) :: sigma)%list const.
+Proof.
+intros sigma const a ty h.
+induction const.
+- apply sat_nil.
+- destruct a0. apply sat_cons.
+  + apply IHconst.
+    apply extra_sat_xi with
+    (x := (subst1_ty (a, ty) t, subst1_ty (a, ty) t0)).
+    simpl in h. apply h.
+  + simpl.
+    simpl in h.
+    dependent destruction h.
+    apply H.
+Qed.
+
+(* -- Build -- *)
+
+Inductive build_subst : s_rules -> constraints -> Prop :=
+| build_nil : build_subst List.nil List.nil
+| build_consleft sigma const a ty :
+  build_subst sigma (subst1_const (a, ty) const) ->
+  build_subst ((a, ty) :: sigma)%list ((TVar a, ty) :: const)%list
+| build_consright sigma const b ty :
+  build_subst sigma (subst1_const (b, ty) const) ->
+  build_subst ((b, ty) :: sigma)%list ((ty, TVar b) :: const)%list
+| build_consimp rul sigma const tyA tyB tyC tyD :
+  build_subst (rul :: sigma)%list ((tyC, tyA) :: (tyB, tyD) :: const)%list ->
+  build_subst (rul :: sigma)%list ((TImp tyA tyB, TImp tyC tyD) :: const)%list.
+
+Lemma build_sat : forall (sigma : s_rules) (const : constraints),
+  build_subst sigma const ->
+  good_rules sigma ->
+  sat_xi sigma const.
+Proof.
+intros sigma const h good.
+induction h.
+- apply sat_nil.
+- dependent destruction good.
+  apply sat_cons.
+  + apply subst_sat_xi.
+    apply IHh. apply good.
+  + dependent destruction H.
+* reflexivity.
+* simpl.
+  case_eq (a =? a); intro eq.
+  -- rewrite <- subst1_ty_id.
+     reflexivity.
+     apply good_nFTV. apply H.
+  -- rewrite Nat.eqb_refl in eq.
+     apply Bool.diff_true_false in eq.
+     contradiction.
+- dependent destruction good.
+  apply sat_cons.
+  + apply subst_sat_xi.
+    apply IHh. apply good.
+  + dependent destruction H.
+* reflexivity.
+* simpl.
+  case_eq (b =? b); intro eq.
+  -- rewrite <- subst1_ty_id.
+     reflexivity.
+     apply good_nFTV. apply H.
+  -- rewrite Nat.eqb_refl in eq.
+     apply Bool.diff_true_false in eq.
+     contradiction.
+- assert (sat_xi (rul :: sigma)%list ((tyC, tyA) :: (tyB, tyD) :: const)%list).
+  apply IHh. apply good.
+  apply sat_cons.
+  + apply extra_sat_xi with (x := (tyB, tyD)).
+    apply extra_sat_xi with (x := (tyC, tyA)).
+    apply H.
+  + dependent destruction H.
+    dependent destruction H.
+    rewrite ? dist_subst_ty.
+    rewrite H0. rewrite H1.
+    reflexivity.
+Qed.
+
+(* Bidir *)
+
+Axiom cons_inj : forall {A : Type} (a1 a2 : A) (l1 l2 : list A),
+  (a1 :: l1)%list = (a2 :: l2)%list ->
+  a1 = a2 /\ l1 = l2.
+
+Lemma build_app : forall (const1 const2 : constraints) (sigma : s_rules) ,
+  build_subst sigma (const1 ++ const2)%list ->
+  exists sigma1 sigma2: s_rules,
+  build_subst sigma1 const1 /\
+  build_subst sigma2 (subst_const sigma1 const2) /\
+  sigma = (sigma1 ++ sigma2)%list.
+Proof.
+intros.
+dependent induction H.
+--
+dependent destruction const1; simpl in x.
+- exists List.nil. exists List.nil.
+  rewrite <- x. simpl.
+  split. apply build_nil.
+  split. apply build_nil.
+  reflexivity.
+- discriminate.
+--
+dependent destruction const1;
+dependent destruction const2.
+- simpl in x. discriminate.
+- simpl in x.
+  exists List.nil. simpl.
+  exists ((a, ty) :: sigma)%list.
+  split. apply build_nil.
+  split. rewrite <- x.
+  apply build_consleft. apply H.
+  reflexivity.
+- rewrite List.app_nil_r in x.
+  exists ((a, ty) :: sigma)%list.
+  exists List.nil. simpl. rewrite List.app_nil_r.
+  split. rewrite <- x.
+  apply build_consleft. apply H.
+  split. rewrite subst_const_nil. apply build_nil.
+  reflexivity.
+- simpl in x. apply cons_inj in x. destruct x.
+  assert (
+    exists sigma1 sigma2 : s_rules,
+    build_subst sigma1 (subst1_const (a, ty) const1) /\
+    build_subst sigma2 (subst_const sigma1 (subst1_const (a, ty) (t0 :: const2)%list)) /\
+    sigma = (sigma1 ++ sigma2)%list
+  ). apply IHbuild_subst.
+  rewrite <- app_subst1_const.
+  rewrite <- H1.
+  apply JMeq_refl.
+  destruct H2. destruct H2.
+  exists ((a, ty) :: x)%list.
+  exists x0.
+  split. rewrite <- H0.
+  apply build_consleft. apply H2.
+  split. rewrite <- step_subst_const. apply H2.
+  simpl. destruct H2. destruct H3. rewrite H4.
+  reflexivity.
+--
+dependent destruction const1;
+dependent destruction const2.
+- simpl in x. discriminate.
+- simpl in x.
+  exists List.nil. simpl.
+  exists ((b, ty) :: sigma)%list.
+  split. apply build_nil.
+  split. rewrite <- x.
+  apply build_consright. apply H.
+  reflexivity.
+- rewrite List.app_nil_r in x.
+  exists ((b, ty) :: sigma)%list.
+  exists List.nil. simpl. rewrite List.app_nil_r.
+  split. rewrite <- x.
+  apply build_consright. apply H.
+  split. rewrite subst_const_nil. apply build_nil.
+  reflexivity.
+- simpl in x. apply cons_inj in x. destruct x.
+  assert (
+    exists sigma1 sigma2 : s_rules,
+    build_subst sigma1 (subst1_const (b, ty) const1) /\
+    build_subst sigma2 (subst_const sigma1 (subst1_const (b, ty) (t0 :: const2)%list)) /\
+    sigma = (sigma1 ++ sigma2)%list
+  ). apply IHbuild_subst.
+  rewrite <- app_subst1_const.
+  rewrite <- H1.
+  apply JMeq_refl.
+  destruct H2. destruct H2.
+  exists ((b, ty) :: x)%list.
+  exists x0.
+  split. rewrite <- H0.
+  apply build_consright. apply H2.
+  split. rewrite <- step_subst_const. apply H2.
+  simpl. destruct H2. destruct H3. rewrite H4.
+  reflexivity.
+--
+dependent destruction const1;
+dependent destruction const2.
+- simpl in x. discriminate.
+- simpl in x.
+  exists List.nil. simpl.
+  exists (rul :: sigma)%list.
+  split. apply build_nil.
+  split. rewrite <- x.
+  apply build_consimp. apply H.
+  reflexivity.
+- rewrite List.app_nil_r in x.
+  exists (rul :: sigma)%list.
+  exists List.nil. simpl. rewrite List.app_nil_r.
+  split. rewrite <- x.
+  apply build_consimp. apply H.
+  split. rewrite subst_const_nil. apply build_nil.
+  reflexivity.
+- simpl in x. apply cons_inj in x. destruct x.
+  assert (
+    exists sigma1 sigma2 : s_rules,
+    build_subst sigma1 ((tyC, tyA) :: (tyB, tyD) :: const1)%list /\
+    build_subst sigma2 (subst_const sigma1 (t0 :: const2)%list) /\
+    (rul :: sigma)%list = (sigma1 ++ sigma2)%list
+  ). apply IHbuild_subst. simpl.
+  rewrite H1.
+  apply JMeq_refl.
+  destruct H2. destruct H2.
+  destruct H2. destruct H3.
+  dependent destruction x.
+  dependent destruction H2.
+  exists (s :: x)%list. exists x0.
+  split. rewrite <- H0.
+  apply build_consimp. apply H2.
+  split. rewrite <- step_subst_const. apply H3.
+  rewrite H4. reflexivity.
+Qed.
+
+Lemma build_bidir_good_syn :
+  forall {n : nat} (gamma : context n) (st : sterm n)
+  (ty : type) (const : constraints) (sigma : s_rules),
+  is_bidir_syn gamma st ty const ->
+  build_subst sigma const ->
+  good_rules sigma
+
+with build_bidir_good_chk :
+  forall {n : nat} (gamma : context n) (ct : cterm n)
+  (ty : type) (const : constraints) (sigma : s_rules),
+  is_bidir_chk gamma ct ty const ->
+  build_subst sigma const ->
+  good_rules sigma.
+
+Proof.
+- intros n gamma st ty const sigma hb h.
+  dependent induction hb.
+  + apply IHhb. apply h.
+  + apply build_bidir_good_chk with
+    (n := n) (gamma := gamma) (ct := ct)
+    (ty := (TVar a)) (const := const).
+    apply H. apply h.
+- intros n gamma st ty const sigma hb h.
+  dependent induction hb.
+  + dependent destruction h. apply good_nil.
+  + apply build_app in h.
+    destruct h.
+    destruct H0.
+    destruct H0.
+    destruct H1.
+    rewrite H2.
+    apply good_app.
+    apply build_bidir_good_chk with
+    (n := n) (gamma := gamma) (ct := ct1)
+    (ty := TImp ty1 ty2) (const := const1).
+    apply hb. apply H0.
+    apply build_bidir_good_syn with
+    (n := m) (gamma := delta) (st := st2)
+    (ty := ty1) (const := const2). (* (const := (subst_const x const2)). *)
+    apply H. admit.
+  + admit.
+Admitted.
+
+(* End goal *)
+
+Lemma add_sat_xi : forall (sigma : s_rules) (rul : s_rule) (const : constraints),
+  sat_xi sigma const -> sat_xi (rul :: sigma)%list const.
+Proof.
+intro sigma.
+induction sigma; intros.
+- apply taut_sat_xi.
+  apply nil_sat_taut.
+  apply H.
+- admit.
+Admitted.
+
+Lemma join_sat_xi : forall (sigma1 sigma2 : s_rules) (const : constraints),
+  sat_xi sigma1 const \/ sat_xi sigma2 const -> sat_xi (sigma1 ++ sigma2)%list const.
+Proof.
+intros. destruct H.
+--
+induction sigma2.
+- rewrite List.app_nil_r. apply H.
+- induction sigma1.
+  + simpl.
+
+Admitted.
+
+Theorem build_bidir_mgu_syn :
+  forall {n : nat} (gamma : context n) (st : sterm n)
+  (ty : type) (const : constraints) (sigma : s_rules),
+  is_bidir_syn gamma st ty const ->
+  build_subst sigma const ->
+  is_mgu sigma const
+
+with build_bidir_mgu_chk :
+  forall {n : nat} (gamma : context n) (ct : cterm n)
+  (ty : type) (const : constraints) (sigma : s_rules),
+  is_bidir_chk gamma ct ty const ->
+  build_subst sigma const ->
+  is_mgu sigma const.
+
+Proof.
+
+--
+
+intros.
+dependent induction H.
+- apply IHis_bidir_syn. apply H0.
+- apply build_bidir_mgu_chk with (n := n) (gamma := gamma) (ct := ct) (ty := (TVar a)).
+  apply H. apply H0.
+
+--
+
+intros.
+dependent induction H.
+---
+split. apply sat_nil.
+dependent destruction H0. simpl.
+intro sigma'. exists sigma'.
+reflexivity.
+---
+apply build_app in H1.
+destruct H1. destruct H1.
+destruct H1. destruct H2.
+rewrite H3.
+split.
+-
+apply app_sat_xi.
+(*
+assert (sat_xi (x0 ++ x)%list const1).
+apply perm_sat_xi with ().
+*)
+admit.
+admit.
+-
+admit.
+---
+admit.
+Admitted.
+
+
+
+
+
+
+
+
+
+
+
+
+
+
+
+
+
+
+
+
+
